First iteration

michael_formal/inference/Learn_EFSM.thy
@@ -4,22 +4,9 @@ begin
 
 declare One_nat_def [simp del]
 
-definition merged_1_8 :: iEFSM where
-  "merged_1_8 = {|
-(0, (0, 1), selectCoke),
-(1, (0, 7), selectPepsi),
-(2, (1, 2), coin50_50),
-(3, (1, 5), coin100_100),
-(4, (2, 3), coin50_100),
-(5, (3, 4), vend_coke),
-(6, (5, 6), vend_coke),
-(7, (7, 1), coin50_50),
-(8, (1, 9), coin50_100),
-(9, (9, 10), vend_pepsi)
-|}"
-
 lemma merge_states_1_8: "merge_states 1 8 pta = merged_1_8"
-  by (simp add: merge_states_def merge_states_aux_def pta_def merged_1_8_def)
+  apply (simp add: merge_states_def merge_states_aux_def pta_def merged_1_8_def)
+  by auto
 
 lemma nondeterministic_pairs_merged_1_8: "nondeterministic_pairs merged_1_8 = {|(1, (2, 9), (coin50_50, 2), coin50_100, 8)|}"
 proof-
@@ -49,15 +36,82 @@ proof-
     apply safe
     by (simp_all add: choices orders)
 qed
+
+definition generator :: generator_function where
+  "generator oldEFSM t1FromOld t1 t2FromOld t2 = (if (oldEFSM, t1FromOld, t1, t2FromOld, t2) = (pta, 1, coin50_50, 8, coin50_100) then None
+                                                  else None)"
+
+definition modifier :: update_modifier where
+  "modifier t1 t2 newFrom newEFSM oldEFSM = (if (t1, t2, newFrom, newEFSM, oldEFSM) = (coin50_50, coin50_100, 1, merged_1_8, pta) then None
+                                             else None)"
          
-value "efsm2dot (tm merged_1_8)"
+lemma merge_1_8: "merge pta 1 8 generator modifier = None"
+proof-
+  have leaves_2_pta: "leaves 2 pta = 1"
+  proof-
+    have set_filter: "Set.filter (\<lambda>x. \<exists>a b ba. x = (2, (a, b), ba)) (fset pta) = {(2, (1, 2), coin50_50)}"
+      apply (simp add: Set.filter_def pta_def)
+      apply safe
+      by (simp_all add: transitions)
+    show ?thesis
+      by (simp add: leaves_def ffilter_def fthe_elem_def Abs_fset_inverse set_filter)
+  qed
+  have leaves_1_8_pta: "leaves 8 pta = 8"
+  proof-
+    have set_filter: "Set.filter (\<lambda>x. \<exists>a b ba. x = (8, (a, b), ba)) (fset pta) = {(8, (8, 9), coin50_100)}"
+      apply (simp add: Set.filter_def pta_def)
+      apply safe
+      by (simp_all add: transitions)
+    show ?thesis
+      by (simp add: leaves_def ffilter_def fthe_elem_def Abs_fset_inverse set_filter)
+  qed
+  have no_direct_subsumption_coin_50_50_coin50_100: "\<not> directly_subsumes (tm pta) (tm merged_1_8) 8 coin50_50 coin50_100"
+    apply (simp add: directly_subsumes_def)
+    apply (rule_tac x="[(''select'', [Str ''pepsi'']), (''coin'', [Num 50])]" in exI)
+    apply standard
+     apply (simp add: accepts_trace_def)
+     apply (rule accepts.step)
+      apply (simp add: step_pta_selectPepsi)
+     apply (rule accepts.step)
+      apply (simp add: step_pta_coin50_7)
+     apply (rule accepts.base)
+    apply standard
+     apply (rule gets_us_to.step_some)
+      apply (simp add: step_pta_selectPepsi)
+     apply (rule gets_us_to.step_some)
+      apply (simp add: step_pta_coin50_7)
+     apply (simp add: gets_us_to.base)
+    apply (simp add: anterior_context_def)
+    apply (simp add: step_merged_1_8_selectPepsi step_merged_1_8_coin50_7)
+    by (simp add: posterior_selectPepsi posterior_coin50_50 no_subsumption_coin50_50_coin50_100)
+  have no_direct_subsumption_coin50_100_coin_50_50: "\<not> directly_subsumes (tm pta) (tm merged_1_8) 1 coin50_100 coin50_50"
+    apply (simp add: directly_subsumes_def)
+    apply (rule_tac x="[(''select'', [Str ''coke''])]" in exI)
+    apply standard
+     apply (simp add: accepts_trace_def)
+     apply (rule accepts.step)
+      apply (simp add: step_pta_selectCoke)
+     apply (rule accepts.base)
+    apply standard
+     apply (rule gets_us_to.step_some)
+      apply (simp add: step_pta_selectCoke)
+     apply (simp add: gets_us_to.base)
+    apply (simp add: anterior_context_def)
+    apply (simp add: step_merged_1_8_selectCoke)
+    by (simp add: posterior_selectCoke no_subsumption_coin50_100_coin50_50)
+  have merge_transitions: "merge_transitions pta merged_1_8 1 8 1 2 9 coin50_50 2 coin50_100 8 generator modifier True = None"
+    apply (simp add: merge_transitions_def easy_merge_def)
+    by (simp add: generator_def modifier_def no_direct_subsumption_coin_50_50_coin50_100
+                     no_direct_subsumption_coin50_100_coin_50_50)
+  show ?thesis
+    apply (simp add: merge_def merge_states_1_8 nondeterminism_def nondeterministic_pairs_merged_1_8)
+    apply (simp add: leaves_2_pta leaves_1_8_pta merge_transitions)
+    by (simp add: nondeterminism_def nondeterministic_pairs_merged_1_8)
+qed
 
-lemma "merge pta 1 8 (\<lambda>a b c d e. Some t) (\<lambda>a b c d e. Some e') = Some b"
-  apply (simp add: merge_def merge_states_1_8 nondeterminism_def nondeterministic_pairs_merged_1_8)
 
-
-lemma "learn traces naive_score (\<lambda>a b c d e. Some t) (\<lambda>a b c d e. Some e') = drinks"
-  apply (simp add: learn_def build_pta scoring_1)
+lemma "learn traces naive_score generator modifier = drinks"
+  apply (simp add: learn_def build_pta scoring_1 merge_1_8)
   sorry
 
 end
